Trident.lean
@@ -1,7 +1,10 @@
-import SSA
-
-namespace Trident.Test
-
-#eval 1 + 1
-
-end Trident.Test
+import Trident.Common.Values
+import Trident.Common.Memory
+import Trident.Common.Smallstep
+import Trident.Source.Lang
+import Trident.Source.Specs.VectorAddSpec
+import Trident.Target.Dialect
+import Trident.Target.Semantics
+import Trident.Target.Parser
+import Trident.Compiler
+import Trident.Proofs.VectorAddProof
